more progress on executable logs

coq/logs.v
@@ -11,16 +11,150 @@ Unset Printing Implicit Defensive.
 (* Implementation of the mutator/collector logs and their execution *)
 Section CollectorLog.
 
-Inductive ActionKind : Set := T | M | A.
+Inductive ActionKind : Set := T | M | A of nat.
+
 Record LogEntry : Set := Entry {
   kind    : ActionKind;
   source  : ptr;
   fld     : nat;
   old     : ptr;
   new     : ptr }.
+
 Definition log := seq LogEntry.
 
+(* A set of pointers *)
+Definition ptr_set := ptrmap_pcm_Encoded unit_st_Encoded.
 
+Section ExecuteLogs.
+
+(* 
+
+It reflect boolean condition into a certificate of type P via the
+function g, and then uses the obtained certificate in the continuation
+f. If the boolean check is failed, the result is undefined, hence both
+the condK combinator and its argument f have the result type option.
+
+*)
+Definition condK P R (c : bool) 
+  (g : is_true c -> P) (f : P -> option R) := 
+  (if c as z return _ = z -> _ 
+   then fun (efl : c = true) => f (g efl)
+   else fun _ => None) (erefl _). 
+
+Lemma condKE P R (c : bool) (g : is_true c -> P) (f : P -> option R) :
+  c -> exists pf, condK g f = f pf.
+Proof.
+rewrite /condK=>X; by suff Z: c = true by subst c; eexists.
+Qed.
+
+(*
+
+The following function executeLog is partial and certified:
+
+- If it returns None, then something must have gone wrong, because the
+  log was malformed (TODO: define a check for good logs).
+
+- If the result is Some (h, g), then h is the resulting heap and g is
+  its new graph certificate, which is threaded through the execution.
+
+*)
+
+Record ExecuteResult := ExRes {hp : heap; gp : graph hp}.
+
+Fixpoint executeLog (h : heap) (g : graph h) (l : log) : 
+    option ExecuteResult := match l with 
+
+  (* Empty log - return heap and its graph certificate *)    
+  | [::] => Some (ExRes g)
+
+  (* Check for allocation with new graph certificate *)
+  | (Entry (A fnum) x _ _ _) :: ls => 
+      condK (@allocG h g x fnum) (fun g' => executeLog g' ls)
+
+  (* Check for modification with new graph certificate *)
+  | (Entry M x fld old new) :: ls =>
+      condK (@modifyG h g x fld new) (fun pf => executeLog (proj1 pf) ls)
+  (* Tracing entry - don nothing *)
+  | (Entry T _ _ _ _) :: ls => executeLog g ls
+  end.
+
+
+(* 
+
+We next define the "good" logs, which lead to consistent
+executions. The definition is recursive and is parametrized by the set
+"obs" of already allocated objects, which also serves as an
+accumulator.
+
+ *)
+
+
+Fixpoint goodLog (obs : seq ptr) (l : log) : bool := match l with 
+  (* Empty log is good *)    
+  | [::] => true
+
+  (* Allocation *)
+  | (Entry (A fnum) x _ _ _) :: ls => 
+      (x != null) && (x \notin obs)      && 
+      goodLog (x :: obs) ls
+      
+  (* Modification *)
+  | (Entry M x fld old new) :: ls =>
+      (old \in [predU pred1 null & obs]) &&
+      (new \in [predU pred1 null & obs]) && 
+      goodLog obs ls                                  
+
+  (* Tracing entry *)
+  | (Entry T x fld old new) :: ls => 
+      (old \in [predU pred1 null & obs]) &&
+      (new \in [predU pred1 null & obs]) &&
+      goodLog obs ls
+  end.
+
+(* The following theorem states that good logs are good for execution *)
+
+Theorem goodToExecute h (g: graph h) (l : log) :
+  goodLog (keys_of h) l -> exists er, executeLog g l = Some er.
+Proof.
+elim: l h g=>[|e ls]G h g; first by eexists.
+case: e=>k x fld old new/=; case: k=>/=[||fnum]; first by case/andP=>_ H; apply: G.
+
+- case/andP=>/andP[H1 H2 H3].
+  have X: (new \in dom h) || (new == null) by rewrite !inE/= orbC keys_dom in H2.
+  case: (condKE (modifyG g x fld (new:=new)) 
+        (fun pf => executeLog (proj1 pf) ls) X)=>/=[[g' H4]]; move=>->.
+  apply: G.
+(* TODO: Use H3 and prove the equality of domains... *)
+  admit.  
+
+case/andP=>/andP[H1]H2 H3.
+have X: (x != null) && (x \notin dom h) by rewrite -keys_dom H1 H2.
+
+case: (condKE (allocG g fnum) (fun pf => executeLog pf ls) X)=>/=[g']->.
+apply: G.
+(* TODO: Use H3 and prove another equality of domains... *)
+
+
+
+
+
+
+
+
+
+(* TODO:
+
+- Define a "good" logs wrt. initial g-heap and a set of objects
+  (recursively) [DONE].
+
+- Prove a lemma, stating that executing a good log leads to the graph
+  [IN PROGRESS].
+
+- Implement the basic expose (apex) function
+
+*)
+
+End ExecuteLogs.
 
 
 
